Priority Queue - Attempt

Max Heapify/max_heapify_2.py
@@ -1,0 +1,13 @@
+def max_heapify(arr):
+    n = len(arr)
+    for i in range(n - 1, -1, -1):
+        swim_up(arr, i)
+
+def swim_up(arr, i):
+    while i > 0 and arr[i] > arr[(i - 1) // 2]:
+        arr[i], arr[(i - 1) // 2] = arr[(i - 1) // 2], arr[i]
+        i = (i - 1) // 2
+        
+arr = [4, 10, 3, 5, 1]
+max_heapify(arr)
+print(arr)
