Max Heapify/max_heapify_2.dfy
@@ -1,0 +1,46 @@
+method max_heapify(pq: array<int>)
+    requires pq.Length > 0
+    ensures multiset(pq[..]) == old(multiset(pq[..]))
+    ensures is_max_heap(pq)
+    modifies pq
+{
+    var i := pq.Length - 1;
+    while (i >= 0)
+        invariant -1 <= i <= pq.Length - 1
+        invariant multiset(pq[..]) == old(multiset(pq[..]))
+    {
+        swim(pq, i);
+        i := i - 1;
+    }
+}
+
+method swim(pq: array<int>, k: nat)
+    requires pq.Length > 0
+    requires 0 <= k <= pq.Length - 1
+    requires is_swimmed(pq, pq.Length - 1)
+    ensures multiset(pq[..]) == old(multiset(pq[..]))
+    modifies pq
+{
+    var i := k;
+    while (i > 0 && pq[i] > pq[(i - 1) / 2])
+        invariant 0 <= i <= k
+        invariant multiset(pq[..]) == old(multiset(pq[..]))
+        invariant is_swimmed(pq, i)
+    {
+        pq[i], pq[(i - 1) / 2] := pq[(i - 1) / 2], pq[i];
+        i := (i - 1) / 2;
+    }
+}
+
+predicate is_swimmed(pq: array<int>, k: nat)
+    reads pq
+{
+    (forall i :: 1 <= i < pq.Length && i != k ==> pq[(i - 1) / 2] >= pq[i]) &&
+	(k > 0 ==> forall i :: 1 <= i < pq.Length && (i - 1) / 2 == k ==> pq[((i - 1) / 2 - 1) / 2] >= pq[i])
+}
+
+predicate is_max_heap(pq: array<int>)
+    reads pq
+{
+    forall i :: 1 <= i < pq.Length ==> pq[(i - 1) / 2] >= pq[i]
+}
