Priority Queue/priority_queue.dfy
@@ -1,0 +1,105 @@
+/*
+Credit: João Carlos Pascoal Faria
+Source: https://github.com/joaopascoalfariafeup/DafnyProjects/blob/main/PriorityQueue.dfy
+*/
+
+
+class {:autocontracts} PriorityQueue {
+	// Private variables
+  	var pq: array<int>;
+  	var size : nat;
+
+  	const smallest_size := 2;
+
+ 
+	// Public methods
+  	constructor ()
+  	{
+		pq := new int[smallest_size];
+		this.size := 0; 
+  	}
+
+	predicate method is_empty()
+	{
+		size == 0
+	}
+
+	method insert(x : int)
+		ensures multiset(pq[..size]) == old(multiset(pq[..size])) + multiset{x}
+	{
+		if size == pq.Length {
+			resize();
+		}
+
+		pq[size] := x;
+		size := size + 1;
+
+		swim();
+	}
+
+	method max() returns (x: int)
+		requires is_empty() == false
+	{
+		return pq[0];
+	}
+
+
+	// Private helper methods
+	method resize()
+		requires size == pq.Length
+		ensures pq[..size] == old(pq[..size])
+		ensures pq.Length > size
+	{
+		var temp := pq;
+		var new_size := 2 * size;
+		if (size < smallest_size)
+		{
+			new_size := smallest_size;
+		}
+		pq := new int[new_size];
+		forall i | 0 <= i < temp.Length {
+			pq[i] := temp[i];
+		}
+	}
+
+
+	method {:autocontracts false} swim()
+		requires size > 0
+		requires is_swimmed(size - 1)
+		ensures multiset(pq[..size]) == old(multiset(pq[..size]))
+		ensures is_max_heap()
+		modifies pq
+	{
+		var k := size - 1;
+		while (k > 0 && pq[k] > pq[(k - 1) / 2])
+			invariant 0 <= k <= size - 1
+			invariant is_swimmed(k)
+			invariant multiset(pq[..size]) == old(multiset(pq[..size]))
+		{
+			pq[k], pq[(k - 1) / 2] := pq[(k - 1) / 2], pq[k];
+			k := (k - 1) / 2;
+		}
+	}
+ 
+	predicate {:autocontracts false} is_swimmed(k: nat)
+		reads pq
+		reads this
+	{
+		(size <= pq.Length) &&
+		(forall i :: 1 <= i < size && i != k ==> pq[(i - 1) / 2] >= pq[i]) &&
+		(k > 0 ==> forall i :: 1 <= i < size && (i - 1) / 2 == k ==> pq[((i - 1) / 2 - 1) / 2] >= pq[i])
+	}
+
+	predicate Valid()
+	{
+		is_max_heap()
+	}
+ 
+	predicate {:autocontracts false} is_max_heap()
+		reads pq
+		reads this
+	{
+		(size <= pq.Length) &&
+		(forall i :: 1 <= i < size ==> pq[(i - 1) / 2] >= pq[i])
+	}
+}
